

### Poisson Distribution:

Suppose that an experiment with two possible outcomes  $S$  and  $f$  and  $P(S) = P$  and  $P(f) = 1-P$  is repeated independently and indefinitely. Let  $P$  be small ( $P \rightarrow 0$ ), such that  $np \rightarrow \lambda$  as  $n \rightarrow \infty$ . Then, the probability distribution of the number of successes is

$$P(X=x) = \frac{e^{-\lambda} \lambda^x}{x!}; \quad x = 0, 1, 2, \dots, \infty.$$

Which is called as poisson distribution with parameter  $\lambda$ .

### Derivation:-

The probability of  $x$  successes in  $n$  trials in the binomial distribution  $b(x; n, p)$  is given by

$$\begin{aligned} P(X=x) &= \binom{n}{x} p^x q^{n-x} \\ &= \frac{n(n-1)\dots(n-x+1)(n-x)!}{(n-x)! x!} p^x q^{n-x} \\ &= \frac{n(n-1)(n-2)\dots(n-x+1)}{x!} p^x q^{n-x} \end{aligned}$$

Let  $np = \lambda$ ,  $\Rightarrow p = \frac{\lambda}{n}$  and  $q = (1 - \frac{\lambda}{n})$   
replacing  $p$  and  $q$  in terms of  $\lambda$ .  $\Rightarrow$

$$P(X=x) = \frac{n(n-1)\dots(n-x+1)}{x!} \left(\frac{\lambda}{n}\right)^x \left(1 - \frac{\lambda}{n}\right)^{n-x}$$

$$P(X=x) = \frac{\lambda^x}{x!} \cdot \frac{n(n-1)\dots(n-x+1)}{n^x} \cdot \left(1 - \frac{\lambda}{n}\right)^n \cdot \left(1 - \frac{\lambda}{n}\right)^{-x}$$

$$\begin{aligned}
 x) &= \frac{\lambda^x}{x!} \frac{n^x}{n^x} \cdot \left[ \left(1 - \frac{1}{n}\right) \left(1 - \frac{2}{n}\right) \dots \left(1 - \frac{x-1}{n} + \frac{1}{n}\right) \right] \cdot \left(1 - \frac{\lambda}{n}\right)^n \left(1 - \frac{\lambda}{n}\right)^{-x} \\
 &= \frac{\lambda^x}{x!} \cdot \left[ \left(1 - \frac{1}{n}\right) \left(1 - \frac{2}{n}\right) \dots \left(1 - \frac{x-1}{n}\right) \right] \left(1 - \frac{\lambda}{n}\right)^n \left(1 - \frac{\lambda}{n}\right)^{-x}
 \end{aligned}$$

Since  $\lambda$  remains fixed and  $n$  becomes large we observe that each of the term.

$$\left[ \left(1 - \frac{1}{n}\right) \left(1 - \frac{2}{n}\right) \dots \left(1 - \frac{x-1}{n}\right) \right] \rightarrow 1 \quad \text{and}$$

$$\left(1 - \frac{\lambda}{n}\right)^x \rightarrow 1 \quad \text{for large } n.$$

$$P(X=x) = \frac{\lambda^x}{x!} \left(1 - \frac{\lambda}{n}\right)^n$$

$$\text{The term } \left(1 - \frac{\lambda}{n}\right)^n = \left[ \left(1 - \frac{\lambda}{n}\right)^{\frac{n}{\lambda}} \right]^\lambda$$

$$\therefore k = \frac{n}{\lambda}$$

$$\frac{\lambda}{n} = \frac{1}{k}$$

$$\left(1 - \frac{\lambda}{n}\right)^n = \left[ \left(1 - \frac{1}{k}\right)^k \right]^\lambda$$

If  $n$  increases indefinitely, so for each  $k$ ,

$$\left[ \left(1 - \frac{1}{k}\right)^k \right] \text{ tends to } e^{-1} \quad \text{where } e = 2.71828$$

Thus

$$\left[ \left(1 - \frac{1}{k}\right)^k \right]^\lambda \rightarrow e^{-\lambda}$$

$$\Rightarrow \lim_{n \rightarrow \infty} P(X=x) = \lim_{n \rightarrow \infty} \frac{\lambda^x}{x!} \left[ \left(1 - \frac{1}{k}\right)^k \right]^\lambda$$

$$= \frac{\lambda^x}{x!} \lim_{n \rightarrow \infty} \left[ \left(1 - \frac{1}{k}\right)^k \right]^\lambda$$

$$P(X=x) = \frac{\lambda^x}{x!} e^{-\lambda}$$

$$\therefore \lim_{n \rightarrow \infty} \left(1 - \frac{1}{k}\right)^k = e^{-1}$$

$$k = \frac{n}{\lambda}$$

moments:

Let  $X$  be a random variable with the Poisson distribution  $P(X; \lambda)$  then.

$$\mu'_r = E(X^r) = \sum_{X=0}^{\infty} X^r P(X; \lambda)$$

$$\underline{r=1} \quad \mu'_1 = \sum_{X=0}^{\infty} X \cdot \frac{e^{-\lambda} \lambda^X}{X!} \quad ; \quad X = 0, 1, 2, \dots, \infty.$$

$$= e^{-\lambda} \sum_{X=0}^{\infty} \frac{X \lambda^X}{X!}$$

$$= e^{-\lambda} \left[ 0 + 1 \cdot \frac{\lambda}{1!} + 2 \cdot \frac{\lambda^2}{2!} + 3 \cdot \frac{\lambda^3}{3!} + \dots \right]$$

$$= e^{-\lambda} \left[ \lambda + \lambda^2 + \frac{\lambda^3}{2!} + \frac{\lambda^4}{3!} + \dots \right]$$

$$= \lambda e^{-\lambda} \left[ 1 + \lambda + \frac{\lambda^2}{2!} + \frac{\lambda^3}{3!} + \dots \right]$$

$$= \lambda e^{-\lambda} \cdot e^{\lambda} \quad \therefore \left[ e^{\theta} = 1 + \theta + \frac{\theta^2}{2!} + \frac{\theta^3}{3!} + \dots \right]$$

$$\boxed{\mu'_1 = \lambda} = \text{Mean} = E[X]$$

$$\mu'_2 = E[X^2] = E[X(X-1) + X] = E[X(X-1)] + E[X]$$

$$= E[X(X-1)] + \lambda.$$

$$E[X(X-1)] = \sum_{X=0}^{\infty} X(X-1) \frac{e^{-\lambda} \lambda^X}{X!}$$

$$= e^{-\lambda} \left[ 0 + 0 + 2 \cdot 1 \cdot \frac{\lambda^2}{2!} + 3 \cdot 2 \cdot \frac{\lambda^3}{3!} + 4 \cdot 3 \cdot \frac{\lambda^4}{4!} + 5 \cdot 4 \cdot \frac{\lambda^5}{5!} + \dots \right]$$

$$= \lambda^2 e^{-\lambda} \left[ 1 + \frac{\lambda}{1!} + \frac{\lambda^2}{2!} + \frac{\lambda^3}{3!} + \dots \right]$$

$$= \lambda^2 e^{-\lambda} \cdot e^{\lambda} = \boxed{\lambda^2 = E[X(X-1)]}$$



$$E(x^2) = \lambda + \lambda^2$$

$$\mu_3' = E[x^3] = E[x(x-1)(x-2) + 3x(x-1) + x]$$

$$= E[x(x-1)(x-2)] + 3E[x(x-1)] + E[x]$$

$$= E[x(x-1)(x-2)] + 3[\lambda^2] + \lambda$$

$$E[x(x-1)(x-2)] = \sum_{x=0}^{\infty} x(x-1)(x-2) \frac{e^{-\lambda} \lambda^x}{x!}$$

$$= e^{-\lambda} \left[ \frac{3 \cdot 2 \cdot 1 \lambda^3}{3!} + \frac{4 \cdot 3 \cdot 2 \lambda^4}{4!} + \frac{5 \cdot 4 \cdot 3 \lambda^5}{5!} + \frac{6 \cdot 5 \cdot 4 \lambda^6}{6!} + \dots \right]$$

$$= e^{-\lambda} \left[ \lambda^3 + \frac{\lambda^4}{1!} + \frac{\lambda^5}{2!} + \frac{\lambda^6}{3!} + \dots \right]$$

$$= \lambda^3 e^{-\lambda} \left[ 1 + \frac{\lambda}{1!} + \frac{\lambda^2}{2!} + \frac{\lambda^3}{3!} + \dots \right]$$

$$= \lambda^3 e^{-\lambda} e^{\lambda}$$

$$E[x(x-1)(x-2)] = \lambda^3$$

$$\mu_3' = \lambda^3 + 3\lambda^2 + \lambda$$

$$\mu_4' = E[x^4] = E[x(x-1)(x-2)(x-3) + 6x(x-1)(x-2) + 7x(x-1) + x]$$

$$\mu_4' = E[x(x-1)(x-2)(x-3)] + 6\lambda^3 + 7\lambda^2 + \lambda$$

$$[X(X-1)(X-2)(X-3)]$$

$$= \sum_{x=0}^{\infty} X(X-1)(X-2)(X-3) \frac{e^{-\lambda} \lambda^x}{x!}$$

$$= e^{-\lambda} \left[ 4 \cdot 3 \cdot 2 \cdot 1 \frac{\lambda^4}{4!} + 5 \cdot 4 \cdot 3 \cdot 2 \frac{\lambda^5}{5!} + 6 \cdot 5 \cdot 4 \cdot 3 \frac{\lambda^6}{6!} + 7 \cdot 6 \cdot 5 \cdot 4 \frac{\lambda^7}{7!} + \dots \right]$$

$$= \lambda^4 e^{-\lambda} \left[ 1 + \frac{\lambda}{1!} + \frac{\lambda^2}{2!} + \frac{\lambda^3}{3!} + \dots \right]$$

$$= \lambda^4 e^{-\lambda} e^{\lambda}$$

$$= \lambda^4 = E[X(X-1)(X-2)(X-3)]$$

$$\Rightarrow \mu_4' = \lambda^4 + 6\lambda^3 + 7\lambda^2 + \lambda$$

Moments about Mean :

$$\mu_1'' = \mu_1' - \mu_1' = 0 \quad (\text{always})$$

$$\begin{aligned} \mu_2'' &= \mu_2' - \mu_1'^2 \\ &= \lambda^2 + \lambda - \lambda^2 \end{aligned}$$

$$\boxed{\mu_2'' = \lambda} = \text{Var}(X) \Rightarrow \boxed{\text{S.D} = \sqrt{\lambda}}$$

$$\begin{aligned} \mu_3'' &= \mu_3' - 3\mu_2' \mu_1' + 2\mu_1'^3 \\ &= (\lambda^3 + 3\lambda^2 + \lambda) - 3(\lambda^2 + \lambda)(\lambda) + 2\lambda^3 \\ &= \lambda^3 + 3\lambda^2 + \lambda - 3\lambda^3 - 3\lambda^2 + 2\lambda^3 \end{aligned}$$

$$\boxed{\mu_3'' = \lambda}$$

$$\begin{aligned}
 \mu_4' &= \mu_4' - 4\mu_3'\mu_1' + 6\mu_2'\mu_1'^2 - 3\mu_1'^4 \\
 &= (\lambda^4 + 6\lambda^3 + 7\lambda^2 + \lambda) - 4\lambda(\lambda^3 + 3\lambda^2 + \lambda) \\
 &\quad + 6\lambda^2(\lambda^2 + \lambda) - 3\lambda^4 \\
 &= \cancel{\lambda^4} + 6\lambda^3 + 7\lambda^2 + \lambda - 4\lambda^4 - 12\lambda^3 - 4\lambda^2 \\
 &\quad + 6\lambda^4 + 6\lambda^3 - 3\lambda^4
 \end{aligned}$$

$$\mu_4 = 3\lambda^2 + \lambda$$

Measure of Skewness

$$\beta_1 = \frac{\mu_3}{\mu_2^3} = \frac{\lambda^2}{\lambda^3} = \frac{1}{\lambda} \Rightarrow \boxed{\beta_1 = \frac{1}{\lambda}}$$

$$\beta_2 = \frac{\mu_4}{\mu_2^2} = \frac{3\lambda^2 + \lambda}{\lambda^2} = 3 + \frac{1}{\lambda}$$

$$\boxed{\beta_2 = 3 + \frac{1}{\lambda}}$$

Measure of Kurtosis

$$\gamma_1 = \sqrt{\beta_1} = \sqrt{\frac{1}{\lambda}} = \boxed{\frac{1}{\sqrt{\lambda}} = \gamma_1}$$

$$\gamma_2 = \beta_2 - 3 = 3 + \frac{1}{\lambda} - 3$$

$$\boxed{\gamma_2 = \frac{1}{\lambda}}$$

## Poisson

Q8

A secretary makes 2 typing errors per page on the average. What is the probability that on the next page she makes

- a) 4 or more errors      b) no errors  
c) At least 2 errors.

Sol:

a)  $P(X \geq 4)$

Mem =  $\lambda = 2$

$$= \sum_{x=4}^{\infty} P(X; 2) = 1 - P(X < 4)$$

$$= 1 - \sum_{x=0}^3 P(X; 2)$$

$$= 1 - 0.8571$$

$$= 0.1429$$

b)  $P(X=0) = P(0; 2) = \frac{e^{-\lambda} \lambda^x}{x!} = \frac{e^{-2} 2^0}{0!} = e^{-2} = 0.1353$

c)  $P(X \geq 2) = 1 - P(X < 2) = 1 - \sum_{x=0}^1 P(X; 2)$

$$= 1 - \left( \frac{e^{-2} 2^0}{0!} + \frac{e^{-2} 2^1}{1!} \right)$$

$$= 1 - 0.1353 - 0.2707$$

$$= 1 - 0.4060$$

$$= 0.5940$$



# OF POISSON DISTRIBUTION:

Ques:

The Distribution of typing mistakes committed by a typist is given below. a) Assuming poisson model, find out the expected frequencies

Mistakes per page	0	1	2	3	4	5
No. of pages	142	156	69	27	5	1

Sol:

$$\text{Mean} = \frac{\sum fx}{\sum f} = \frac{400}{400} = 1 = \lambda = np.$$

$$f(x) = NP(x) = 400 \times \frac{e^{-\lambda}}{x!}; \quad x = 0, 1, 2, \dots, 5$$

$$P(0) = e^{-\lambda} = e^{-1} = 0.3679$$

X	$P(x) = \frac{e^{-\lambda} \lambda^x}{x!}$	Expected frequency $f(x) = NP(x)$
0	0.3679	$400 \times 0.3679 = 147$
1	0.3679	$147.16 \approx 147$
2	$\frac{0.3679 \times 1^2}{2!} = 0.18395$	$73.58 \approx 74$
3	$0.3679 / 3! = 0.061317$	$24.52 \approx 25$
4	$0.3679 / 4! = 0.01533$	$6.13 \approx 6$
5	$0.3679 / 5! = 0.003066$	$1.22 \approx 1$

- b) Is the skewness between observed and Expected data set remains same
- c) Is the data set skewed
- b) Does observed and Expected data suggests equal skewness and Kurtosis?



Q7. On the average a certain intersection results in 3 traffic accidents per month. What is the probability that in any given month at this intersection.

- a) exactly 5 accidents will occur?
- b) Less than 3 accidents will occur?
- c) at least 2 accidents will occur?

Sol:

$$\bar{x} = 3 \Rightarrow \mu p = \boxed{3 = \lambda}$$

we have to find

$$a) P(X=5, \lambda=3) = \sum_{x=0}^5 P(x; \lambda) - \sum_{x=0}^4 P(x; \lambda)$$

=

$$= 0.1008 //$$

$$b) P(X < 3)$$

$$= \sum_{x=0}^2 P(x; \lambda) = 0.4232$$

$$c) P(X \geq 2)$$

$$= 1 - \sum_{x=0}^1 P(x; \lambda) = 1 - 0.1991 = 0.8009$$